Basics
=========

~~~haskell
    t   ::= s                   -- sort (either '*' or '<>')
        |   x                   -- variable
        |   (a b)               -- application
        |   (\ (x: A) := e)     -- abstraction
        |   (all (x: A): B)     -- dependent product
~~~


Typing relation:

~~~
    Gamma |- t : T
~~~

means that in context `Gamma` the term `t` has type `T`.




~~~
    Axiom:

    [] |- * : <>
~~~



~~~
    Variable:

    Gamma |- A : *
    x not in Gamma
    ----------------------
    Gamma, (x:A) |- x : A
~~~



~~~
    Weaken:

    Gamma |- t : T
    Gamma |- A : *
    x not in Gamma
    ----------------------
    Gamma, (x:A) |- t : T
~~~



~~~
    Product:

    Gamma |- A : s1
    Gamma, (x:A) |- B : s2
    ----------------------
    Gamma |- (all (x: A): B): s2
~~~



~~~
    Abstraction:

    Gamma, (x:A) |- e : B
    -----------------------------------------
    Gamma |- (\ (x: A) := e): (all (x: A): B)
~~~



~~~
    Application:

    Gamma |- f : (all (x: A): B)
    Gamma |- a : A
    ----------------------
    Gamma |- f a : B[x:=a]
~~~



~~~
    Conversion:

    Gamma |- t : T
    Gamma |- U : s
    T ~> U   or   U ~>  T
    ----------------------
    Gamma |- t : U
~~~



Strong Normalization
====================


Lambda Function Space
---------------------

Let `A` and `B` be set of strongly normalizing lambda terms. We define the
lambda function space between `A` and `B` as the set of lambda terms

~~~
    [A -> B] :=
        {f: f a in B for all a in A}
~~~

Theorem: *All elements of `[A -> B]` are strongly normalizing as long as the
elements of `A` and `B` are strongly normalizing:*

Proof:

Let `f` be an element of `[A -> B]`.

Then by definition of `[A -> B]` the term `f a` must be in `B` for all `a` in
`A`.

Since `A` is saturated, it is not empty.  Therefore there is at least one `f
a` which is in `B`.

Since all elements of `B` are strongly normalizing, the term `f a` is strongly
normalizing.

Since all subterms of a strongly normalizing term are strongly normalizing,
we can conclude that `f` is strongly normalizing.





Saturated Set
-------------

Definition: *A base term is a term of the form `x t1 t2 ... tn` where `x` is a
variable and `t1`, `t2`, ... `tn` are strongly normalizing terms. `n` can be
zero.*


Definition: *A set `S` of terms is saturated if the following conditions are
satisfied:*

- All terms in `S` are strongly normalizing

- `S` contains all base terms

- For all `b` in `S`, `a` is in `SN` and `key-reduce a = b`, then `a` is in
  `S` as well.

The last two conditions are *closure conditions*.


Definition: `SAT` is the set of all saturated sets.


We can saturate a set `S` of strongly normalizing terms.

~~~
    saturate S :=
        least superset of S which contains all base terms and is closed
        under key expansion
~~~

The function `saturate` is a closure operator i.e. it is monotonic, increasing
and idempotent. Therefore the set of all saturated sets `SAT` forms a complete
lattice which has the nice property that arbitrary intersections of saturated
sets are saturated.


Theorem: *If `A` and `B` are saturated sets, then `[A -> B]` is saturated as
well.*

Proof: We have to show that `[A -> B]` satisfies the 3 conditions required to be
saturated set.

1. All elements of `[A -> B]` are strongly normalizing:

   As has been proved above are all elements of `[A -> B]` strongly normalizing
   as long as all elements of `A` and `B` are strongly normalizing.

   Since `A` and `B` are saturated, all their elements are strongly normalizing
   by definition.

2. All base terms must be in `[A -> B]`:

   Remember that a base term has the form `x t1 t2 ... tn` where `x` is a
   variable and `t1`, `t2`, ... are strongly normalizing and `n` can be zero.

   Let `a` be a term of `A`. Then `x t1 t2 ... tn a` is in `B`, because `B`
   contains all base terms.

   Then the term `x t1 t2 ... tn` is in `[A -> B]` by definition of `[A -> B]`.

   Therefore all base terms are in `[A -> B]`.

3. `[A -> B]` must be closed under key expansion:

   Let `e t1 t2 ... tn` be in `[A -> B]`. By definition `e t1 t2 ... tn a` is in
   `B` for all `a` in `A`. Since `A` is not empty there exists an `e t1 t2 ...
   tn a` in `B` for some `a` in `A`.

   Therefore `r t1 t2 ... tn a` is in `B` where `r` is a strongly normalizing
   redex reducing to `e`. Reason: `B` is saturated and therefore closed under
   key expansion.

   By definition of `[A -> B]` the term `r t1 t2 ... tn` is in `[A -> B]`.

   This proves that `[A -> B]` is closed under key expansion.


Summary: The set of saturated sets is closed under forming of arbitrary
intersections and under forming of lambda function spaces.



Kinds
-----

Definition: A *syntactic kind* is a term of one of the forms


~~~
    *

    all (x: A) (y: B) ... : *
~~~

i.e. a kind `K` is a term described by the grammar

~~~
    K   ::=     *
        |       all (x: A): K
~~~

where `K` ranges over kinds, `x` ranges over variables and `A` is an arbitrary
term.


For any term it can be decided by inspection if it is a syntactical kind. From
the definition we see that `K` being a kind implies that `all (x: A): K` is a
kind as well.

In the calculus of constructions it is not possible, that a term reduces to a
kind unless it had been a kind before the reduction. We prove this claim by
showing that all valid syntactical kinds have the type `<>` and all terms of
type `<>` are syntactical kinds.

Both subclaims are sufficient because of the subject reduction property which
states that a reduction does not change its type. So assume that `A ~> K` and
`K` is a kind which has type `<>`. Then by the subject reduction property `A`
must have the same type. This requires that `A` is a syntactical kind if both
subclaims are valid.

It remains to prove the two subclaims.

Theorem: *All valid syntactic kinds `K` have type `<>`*

Proof:

1. `K = *`: Trivial, because `*` has the type `<>`.

2. `K = (all (x: A): B)` and `B` is a kind:

   Since `B` is a kind it has the type `<>`. The product rule states that the
   type of `all (x: A): B` is the type of `B`.




Theorem: *`Gamma |- A: <>` implies that `A` is a syntactical kind.*

Proof by induction on `Gamma |- A: <>`:

- Axiom: `[] |- * : <>`

  Trivial, `*` is a syntactical kind.


- Variable rule: `Gamma |- A : *` implies `Gamma, (x:A) |- x : A`

  This case is not possible, because `A` cannot be `<>`. If it were, it would
  require `Gamma |- <> : *` to be valid which cannot be the case.



- Weaken: `Gamma |- t : T` and `Gamma |- A : *` implies `Gamma, (x:A) |- t : T`

  If `T` is `<>`, then the induction hypothesis already states that `t` is a
  kind.



- Product: `Gamma |- A : s1` and `Gamma, (x:A) |- B : s2` implies `Gamma |- (all
  (x: A): B): s2`

  If `s2 = <>` then the second induction hypothesis states that `B` is a kind.
  This implies that `all (x: A): B` is a kind as well.



- Abstraction: `Gamma |- (all (x: A): B): s` and `Gamma, (x:A) |- e: B` imply
  `Gamma |- (\ (x: A) := e): (all (x: A): B)`

  This case is impossible, because `all (x: A): B` cannot be `<>`.


- Application: `Gamma |- f: all (x: A): B` and `Gamma |- a: A` imply `Gamma |- f
  a: B[x:=a]`

  There are 2 possibilities for `B[x:=a]` is equal to `<>`:

  - `B = <>`: This leads to a contradiction, because the term `all (x: A): <>`
    which is the type of `f` is illegal.

  - `B = x` and `a = <>`: This leads to a contradiction as well, because `Gamma
    |- <> : A` is an invalid typing judgement.


- Conversion: `Gamma |- t : T` and `Gamma |- U: s` and `(T ~> U or U ~> T)`
  imply `Gamma |- t: U`

  This case is impossible because `Gamma |- <>: s` is not a valid typing
  judgement.






Models for a Context
--------------------


A model set is either the set of saturated sets or a function from one model set
to another.

~~~
    ModelSet * :=
        SAT

    ModelSet (all (x: A): B) :=
        {f: ModelSet A -> ModelSet B}, if A is a kind

    ModelSet (all (x: A): B) :=
        ModelSet B,   if A is not a kind
~~~

For each kind, we can define a canonical model

~~~
    canonical-model * :=
        SN

    canonical-model (all (x: A): B) :=
        \ _ := canonical-model B,   if A is a kind

    canonical-model (all (x: A): B) :=
        canonical-model B,  if A is not a kind
~~~



The canonical model of `*` is the set strongly normalizing terms. The canonical
model of `all (x: A): B` depends on whether `A` is a syntactical kind or not. In
the first case it is a function which ignores its argument and returns the
canonical model of `B`. In the second case is the canonical model of `B`.




A model for a context attaches a model to variables.

~~~
    model = [(x1, m1), (x2, m2), ....]
~~~

A model `model` satisfies a valid context `Gamma`, written

~~~
    model |= Gamma
~~~

if it attaches to all constructor variables of the context a model of the model
set of its type (which is a kind by definition of a constructor).

Since there is a canonical model for each syntactic kind, all valid contexts
have a canonical model which satisfies it.


Models for Constructors
-----------------------

~~~
1. Sort:
    model mlist s   :=  SN

2. Variable:
    model mlist x   := mlist x

3. Product
    model mlist (all (x: A): B) :=
        [model mlist A -> model mlist B]        A is no kind

    model mlist (all (x: A): B) :=
        [model mlist A
         -> intersection (m in ModelSet A) (model (mlist + (x,m)) B]
                                                A is a kind
4. Abstraction
    model mlist (\ (x: A) := e) :=
        model mlist e                           A is no kind

    model mlist (\ (x: A) := e) :=
        (m in ModelSet A) |-> model (mlist + (x,m)) e
                                                A is a kind
5. Application
    model mlist (f a) :=
        model mlist f                           a is an object

    model mlist (f a) :=
        (model mlist f) (model mlist a)         a is a constructor
~~~




Models and Substitution
------------------------

~~~
    model mlist B[x:=a] = model mlist B         a is an object

    model mlist B[x:=a]
    = model (mlist + (x, model mlist a)) B      a is a constructor
~~~

Proof: Induction on the structure of `B`:

We prove only the case that `a` is a constructor because it is the more
complicated case.



#### `B` is a Sort

This case is trivial, because `s[x:=a] = s` for any sort `s` and the model of a
sort is always `SN`.


#### `B` is a Variable

*Case `B = y` and `x` and `y` are different:*

~~~
    model mlist y[x:=a]

    = model mlist y                         'x' and 'y' are different

    = mlist y                               definition of 'model'

    = (mlist + (x, model mlist a)) y        'x' and 'y' are different

    = model (mlist + (x, model mlist a)) y  definition of 'model'
~~~


*Case `B = x`:*

~~~
    model mlist x[x:=a]

    = model mlist a

    = (mlist + (x, model mlist a)) x        definition of 'mlist'

    = model (mlist + (x, model mlist a)) x  definition of 'model'
~~~


#### `B` is a Product

Let `B = all (y: C): D`. We prove only the more difficult case that `C` is a
kind.

~~~
    model mlist (all (y: C): D)[x:=a]

    = model mlist (all (y: C[x:=a]): D[x:=a])

    = [model mlist C[x:=a] ->
        intersection
            (m in ModelSet C[x:=a])
            (model (mlist + (y,m)) D[x:=a]]

                definition of 'model'

    = [model (mlist + (x, model mlist a)) C
        intersection
            (m in ModelSet C)
            (model (mlist + (y,m) + (x, model mlist a)) D

                induction hypotheses for 'C' and 'D' and the
                invariance of model sets under substitution

    = model (mlist + (x, model mlist a)) (all (y: C): D)

                definition of 'model'
~~~



#### `B` is an Abstraction

Let `B = (\ (y: C) := e)`. Since `B` is a constructor we know that `e` is a
constructur as well.

We prove only the more difficult case that `C` is a kind.

~~~
    model mlist (\ (y: C) := e)[x:=a]

    = model mlist (\ (y: C[x:=a]) := e[x:=a])

    = (m in ModelSet C[x:=a]) |-> model (mlist + (y,m)) e[x:=a]

            definition of 'model'

    = (m in ModelSet C) |-> model (mlist + (y,m) + (x, model mlist a)) e

            induction hypothesis for 'e' and the invariance of
            'ModelSet' under substitution

    = model (mlist + (x, model mlist a)) (\ (y: C) := e)

            definition of model
~~~


#### `B` is an application

Let `B` = f b`. Since `B` is a constructor we know that `f` must be a
constructor as well.

We prove only the more difficult case that `b` is a constructor.


~~~
    model mlist (f b)[x:=a]


    = model mlist (f[x:=a] b[x:=a])


    = (model mlist f[x:=a]) (model mlist b[x:=a])

            definiton of 'model'

    = (model (mlist + (x, model mlist a)) f)
        (model (mlist + (x, model mlist a)) b)

            induction hypotheses for 'f' and 'b'

    = model (mlist (x, model mlist a)) (f b)

            definition of 'model'
~~~




Models for Constructors
-----------------------

From a model for a valid context we can derive a model for all valid type
constructors in that context.

A term `T` in context `Gamma` is a type constructor, if its type is a kind i.e.
if `Gamma |- T : K` is valid for some kind `K`.

Assume that `m` is a model of context `Gamma` i.e. that `m |= Gamma` is valid.
Then `m` assigns a model to each variable of the context which is a type
constructor i.e. whose type is a kind.

We can extend the model `m` of the context `Gamma` to all terms `T` which are
valid type constructors in that context or are `<>`. I.e. we define a function
`m T` which maps all type constructors `T` in that context to a model of that
type constructor.

We define the function inductively on the structure of `T`.




#### `T` is a Sort`


The model of a sort is the set of strongly normalizing terms.


~~~
    m *  := SN
    m <> := SN
~~~



#### `T` is a Variable


The model of a type constructor variable is exactly the model which `m` assigns
to that variable.



#### `T` is a Product

Now we come to the model of a product `all (x: A): B`. In order to be a type
constructor its type must be a kind. This means that `Gamma |- (all (x: A): B) :
*` must be valid, because the type of a product is always a sort and `*` is the
only sort which is a kind.

According to the typing rules this implies that `Gamma, (x: A) |- B : *` as well
i.e. `B` is a proper type which is a special case of a type constructor with no
arguments.

However for `A` both judgements `A: *` and `A: <>` are possible i.e. `A` can be
a type (constructor) or a kind.

In the first case `x` is not a type constructor variable and therefore the model
`m` is valid for `Gamma` and `Gamma, (x:A)`. In that case we define

~~~
    m (all (x: A): B) :=
        [m A -> m B]

        if A is a proper type
~~~

Since `m` extends naturally to `A` and `B` we define the model of the product to
be the lambda function space between the model of `A` and the model of `B`.

In the second case `x` is a type constructor variable and therefore the model
`m` is not valid for `Gamma, (x: A)` because it does not assign a model to `x`.

Since `A` is a kind, there is a model set `MS := ModelSet A` from which we can
choose an arbitrary element `mx` and append the pair `(x, mx)` to the end of `m`
to get a model for `Gamma, (x: A)`.

We know that such `mx` exists, because a model set is never empty. Unfortunately
it is not unique.

Now we can use the fact that models of types are saturated sets and are
therefore closed under arbitrary intersections. So we define the model of `B` in
the context `Gamma, (x:A)` as

~~~
    m (B, x, A) :=
        intersection { (m, (x,mx)) B | mx in ModelSet AÂ }

        if A is a kind
~~~

where `m, (x,mx)` is the model `m` with the pair `(x,mx)` appended at the end.

Having this definition we can define

~~~
    m (all (x: A): B) :=
        [m A -> m (B, x, A)]

        if A is a kind
~~~


#### `T` is an Abstraction

An that case `T` has the form `\ (x: A) := e` and

~~~
    Gamma |- (\ (x: A) := e): (all (x: A): B)
~~~

must be valid where `B` is a kind (because the product must be a kind).

The fact that `B` is a kind implies that `e` must be a type constructor in the
context `Gamma, (x:A)`.

~~~
    m (\ (x: A) := e) :=
        m e

        if 'A' is a proper type
~~~

~~~
    m (\ (x: A) := e) :=
        function mapping 'mx' from 'ModelSet A' to '(m, (x,mx)) e'

        if 'A' is a kind
~~~


#### `T` is an Application

??????



MISSING:

- `model` preserves substitution

- `model` preserves reduction

Theorem: *The function `model` preserves typesafe substitution with objects,
i.e.*

~~~
    Gamma |- A: *
    Gamma |- K: <>
    Gamma |- a : A
    Gamma, (x:A) |- B : K
    mlist |= Gamma
    -------------------------------------
    model mlist B  =  model mlist B[x:=a]
~~~

Proof by induction on the structure of `B`:


#### `B` is a Sort

This is not possible, because the only valid typing judgement with sorts is `* :
<>` and `<>` is not a kind.



#### `B` is a Variable


If `B` is a variable and `B` is a constructor, then it has to be different from
`x`, because `x` is an object and not a constructor. Therefore the terms `B` and `B[x:=a]` are the same.




#### `B` is a Product

Let `B` be `all (y: C): D`. In that case `K` can only be `*` which implies `D:
*`.

We have to prove the goal

~~~
    model mlist (all (y: C): D)

    = model mlist (all (y: C[x:=a]): D[x:=a])
~~~


We distinguish the cases that `C` is a proper type and `C` is a
kind.


*Case `C` is a proper type:*


~~~
    model mlist (all (y: C): D))

    = [model mlist C -> model mlist D]
                                definition of 'model'

    = [model mlist C[x:=a] -> model mlist D[x:=a]]
                                induction hypotheses

    = model mlist (all (y: C[x:=a]): D[x:=a])
                                definition of 'model'
~~~


*Case `C` is a kind:*

We prove this case the same manner as before. First we expand the definition of
`model`, then we apply the induction hypotheses and then we use the definition
of `model` in backward direction.

~~~
    model mlist (all (y: C): D)

    = [model mlist C -> intersection (model (mlist + (y,my)) D)]
                where 'my in ModelSet C'

    = [model mlist C[x:=a]
      -> intersection (model (mlist + (y,my)) D[x:a])]
                where 'my in ModelSet C'

    = model mlist (all (y: C[x:=a]): D[x:0a])
~~~





#### `B` is an Abstraction

*Case `C` is a proper type:*

~~~
    model mlist (\ (y: C):= e)

    = model mlist e                 definition of 'model'

    = model mlist e[x:=a]           induction hypothesis

    = model mlist (\ (y: C) := e)   definiton of 'model'
~~~

*Case `C` is a kind:*

~~~
    model mlist (\ (y: C):= e)

    = (\ (m: ModelSet C) := model (mlist + (y,m)) e)
                                    definition of 'model'

    = (\ (m: ModelSet C) := model (mlist + (y,m)) e[x:=a])
                                    induction hypothesis

    = model mlist (\ (y: C) := e[x:=a])


    MISSING: 'ModelSet' respects substitution!!!
~~~



#### `B` is an Application

Let `B` be `C D`.







Proof of Normalization
----------------------

Definition: *`Gamma |= t : T` is defined as: For all `(sub, mlist)` such
that `(sub,mlist) |= Gamma` implies `sub t in model mlist T` and `sub
T in SN`.*




Soundness Theorem: *`Gamma |- t : T` implies `Gamma |= t : T`*


Proof by induction of `Gamma |- t : T`:



#### Axiom

We look into the case `[] |- * : <>`.

Since the context is empty, the substitution `sub` and the model list `mlist`
are empty as well.

We have to prove `sub * in model mlist <>` which is equivalent to

~~~
    * in SN
~~~

and trivially valid.





#### Variable

We look into the case `Gamma, (x:A) |- x : A` under the premise `Gamma |- A :
s` for some sort `s` and fresh variable `x`.

We have to prove

~~~
    sub x in model mlist A

    for all (sub,mlist) |= Gamma, (x:A)
~~~

The first condition is trivially satisfied by the definition of `(sub,mlist)
|= Gamma, (x:A)` which is equivalent to the claim.





#### Weaken

We look into the case `Gamma, (x:A) |- t : T` under the premises `Gamma |- t :
T` and `Gamma |- A : s`.

We have to prove

~~~
    sub t in model mlist T

    for all (sub,mlist) |= Gamma, (x:A)
~~~

Let `(sub',mlist')` be `(sub,mlist)` with the entry for `x` removed. This pair
certainly satisfies `Gamma`.

The goal follows mmediately from the induction hypothesis.





#### Product

We look into the case

~~~
    Gamma |- A : s1
    Gamma, (x:A) |- B : s2
    ----------------------
    Gamma |- (all (x: A): B): s2
~~~

and have to prove

~~~
    sub (all (x: A): B) in model mlist s2

    for all (sub,mlist) |= Gamma
~~~

Note that `model mlist s2 = SN` for all sorts by definition.

Furthermore we have

~~~
    sub (all (x: A): B)  =  all (x: sub A): sub B
~~~

which is strongly normalizing if and only if `sub A` and `sub B` are strongly
normalizing.

Since `(sub, mlist) |= Gamma` we can conclude the strong normalization of `sub
A` immediately from the first induction hypothesis.

In case that `A` is not a kind, then `(sub,mlist) |= Gamma, (x:A)` is valid as
well and we can conclude that `sub B` is strongly normalizing immediately from
the second induction hypothesis.

In case that `A` is a kind, which means that `x` is a type constructor variable
we can find a `(sub, mlist + (x,mx)) |= Gamma, (x:A)` for some `mx in ModelSet
A` which is guaranteed to exist, because model sets are always non empty. Then
we can conclude the strong normalization of `sub B` from the second induction
hypothesis.





#### Application

For the case

~~~
    Gamma |- f : (all (x: A): B)
    Gamma |- a : A
    ----------------------------
    Gamma |- f a : B[x:=a]
~~~

we have to prove

~~~
    sub (f a) in model mlist B[x:=a]

    for all (sub,mlist) |= Gamma
~~~

From the induction hypotheses we get

~~~
    sub f in [model mlist A -> model mlist (B, x, A)]

    sub a in model mlist A
~~~

Since `sub (f a) = (sub f) (sub a)` we can conclude

~~~
    sub (f a) in model mlist (B, x, A)
~~~


SUBSTITUTION PROPERTY ???



#### Abstraction

For the case

~~~
    Gamma |- A : s
    Gamma, (x:A) |- e : B
    -----------------------------------------
    Gamma |- (\ (x: A) := e): (all (x: A): B)
~~~

we have to prove

~~~
    sub (\ (x: A) := e) in model mlist (all (x: A): B)

    for all (sub,mlist) |= Gamma
~~~

Note that by definition of `model` we have

~~~
    model mlist (all (x: A): B) = [model mlist A -> model mlist (B, x, A)]
~~~

In order to prove the claim we have to show

~~~
    sub (\ (x: A) := e) a in model mlist (B, x, A)

    for all a in model mlist A
~~~

Since `model mlist (B, x, A)` is a saturated set, it is key expansion closed.
Therefore it is sufficient to prove

~~~
    (sub + (x,a)) e in model mlist (B, x, A)

    sub A in SN
~~~

by using the equality / key reduction

~~~
    sub (\ (x: A) := e) a

    =   (\ (x: sub A) := sub e) a

    ~>  (sub e)[x:=a]

    =   (sub + (x,a) e
~~~

The claim `sub A in SN` follows directly from the induction hypothesis of `Gamma
|- A : s1`.


For the claim `(sub + (x,a)) e in model mlist (B, x, A)` we have to distinguish
the case that `A` is a proper type and `A` is a kind and use the induction
hypothesis of `Gamma, (x:A) |- e : B`.

Case `A` is a proper type:

Since `a in model mlist A` is valid we get `(sub + (x,a), mlist |= Gamma,
(x:A)`.

The induction hypothesis leads to `(sub + (x,a) e in model mlist B` and if `A`
is a proper type, then `model mlist B` is equal to `model mlist (B, x, A)` and
we are done.


Case `A` is a kind:

Here we get

~~~
    (sub + (x,a), mlist + (x,mx)) |= Gamma, (x:A)

    for all mx in ModelSet A
~~~

and the induction hypothesis leads to

~~~
    (sub + (x,a) e in model (mlist + (x,mx)) B

    for all mx in ModelSet A
~~~

i.e. `(sub + (x,a) e` is in the intersection of all `model (mlist + (x,mx) B`
and by definition it is therefore by definition in `model mlist (B, x, A)` and
we are done.









#### Conversion

~~~
    Gamma |- t : T
    Gamma |- U : s
    (T ~> U) or (U ~> T)
    --------------------
    Gamma |- t : U
~~~
